Callee Save Restore working right

src/crypto/loopunroll/testcalleesave.c
@@ -24,6 +24,8 @@
 #include <stdio.h>
 #include <stdint.h> // for uint?_t
 #include "gcc_compat.h"
+#include <inttypes.h>
+
 void __stdcall CalleeSaveRestore(void *one, void *two, void *three, void *four, void *five, void *six, void *seven, void *eight);
 
 uint64_t *one;
@@ -36,14 +38,14 @@ uint64_t *seven;
 uint64_t *eight;
 
 int test_callee_save() {
-  one   = (uint64_t *) malloc(sizeof(uint64_t));
-  two   = (uint64_t *) malloc(sizeof(uint64_t));
-  three = (uint64_t *) malloc(sizeof(uint64_t));
-  four  = (uint64_t *) malloc(sizeof(uint64_t));
-  five  = (uint64_t *) malloc(sizeof(uint64_t));
-  six   = (uint64_t *) malloc(sizeof(uint64_t));
-  seven = (uint64_t *) malloc(sizeof(uint64_t));
-  eight = (uint64_t *) malloc(sizeof(uint64_t));
+  one   = (uint64_t *) malloc(sizeof(uint64_t)); // rax
+  two   = (uint64_t *) malloc(sizeof(uint64_t)); // rsi
+  three = (uint64_t *) malloc(sizeof(uint64_t)); // rdx
+  four  = (uint64_t *) malloc(sizeof(uint64_t)); // rcx
+  five  = (uint64_t *) malloc(sizeof(uint64_t)); // r10
+  six   = (uint64_t *) malloc(sizeof(uint64_t)); // r9
+  seven = (uint64_t *) malloc(sizeof(uint64_t)); // rdi
+  eight = (uint64_t *) malloc(sizeof(uint64_t)); // r8 
 
   *one   = 0x100000000;
   *two   = 0x200000000;
@@ -56,14 +58,16 @@ int test_callee_save() {
 
   CalleeSaveRestore(one, two, three, four, five, six, seven, eight);
 
-  if (*one   != 0x1)   { return 1; }
-  if (*two   != 0x2)   { return 1; }
-  if (*three != 0x3)   { return 1; }
-  if (*four  != 0x4)   { return 1; }  
-  if (*five  != 0x5)   { return 1; }
-  if (*six   != 0x6)   { return 1; }
-  if (*seven != 0x7)   { return 1; }
-  if (*eight != 0x8)   { return 1; }
+  if (*one   != 0x100000000)  { printf("one   is %" PRIu64 "\n", *one);   return 1; }
+  if (*two   != 0x200000000)  { printf("two   is %" PRIu64 "\n", *two);   return 1; }
+  if (*three != 0x300000000)  { printf("three is %" PRIu64 "\n", *three); return 1; }
+  if (*four  != 0x400000000)  { printf("four  is %" PRIu64 "\n", *four);  return 1; }
+  if (*five  != 0x500000000)  { printf("five  is %" PRIu64 "\n", *five);  return 1; }
+  if (*six   != 0x600000000)  { printf("six   is %" PRIu64 "\n", *six);   return 1; }
+  if (*seven != 0x700000000)  { printf("seven is %" PRIu64 "\n", *seven); return 1; }
+  if (*eight != 0x800000000)  { printf("eight is %" PRIu64 "\n", *eight); return 1; }
+
+  return 0;
 }
 
 int __cdecl main(void) {
