src/arch/x64/printMasm.s.dfy
@@ -250,7 +250,7 @@ method printIns(ins:ins)
         case MOVD_xmm_rmm32(dst, src) => print ("  movd "); printXmmOprnd(dst); print(", "); printOprnd(src); print("\n");
         case PCLMULQDQ(dst, src, imm8) => print ("  pclmulqdq "); print(", "); printOprnd(dst); print(", "); printOprnd(src); print(","); printOprnd(imm8); print("\n");
         case VPCLMULQDQ(dst, src1, src2, imm8)  => print ("  vpclmulqdq "); printOprnd(dst); print(", "); printOprnd(src1); print(", "); printOprnd(src2); print(", "); printOprnd(imm8); print("\n");
-        case VMOVDAQ(dst, src)        => print ("  vmovdqa "); printXmmOprnd(dst); print(", "); printOprnd(src); print("\n");          
+        case VMOVDQA(dst, src)        => print ("  vmovdqa "); printXmmOprnd(dst); print(", "); printOprnd(src); print("\n");          
         case VPSHUFD(dst, src, imm8)  => print ("  vpshufd "); print(", "); printOprnd(dst); print(", "); printOprnd(src); print(","); printOprnd(imm8); print("\n");
         case VPXOR(dst, src1, src2)   => print ("  vpxor "); printOprnd(dst); print(", "); printOprnd(src1); print(", "); printOprnd(src2); print("\n");
         case MOVDQA(dst, src)         => print ("  movdqa "); printXmmOprnd(dst); print(", "); printXmmOprnd(src); print("\n");
@@ -259,8 +259,9 @@ method printIns(ins:ins)
         case PSLLD (dst, imm8)        => print ("  pslld ");  printOprnd(dst); print(", "); printOprnd(imm8); print("\n");
         case PSRLDQ(dst, imm8)        => print ("  psrldq "); printOprnd(dst); print(", "); printOprnd(imm8); print("\n");
         case PSRLD (dst, imm8)        => print ("  psrld ");  printOprnd(dst); print(", "); printOprnd(imm8); print("\n");
-        case PUSH (src)               => print ("  push  ");  printOprnd(src); print("\n");
-        case POP (dst)                => print ("  pop  ");   printOprnd(dst); print("\n");
+        case PUSH (src)               => print ("  push  ");  printOprnd64(src); print("\n");
+        case POP (dst)                => print ("  pop  ");   printOprnd64(dst); print("\n");
+        case MOV_m64_imm32(dst,imm32) => print ("  mov  ");  print(", "); printOprnd64(dst); print(","); printOprnd(imm32); print("\n");
 }
 
 method printBlock(b:codes, n:int) returns(n':int)
