src/crypto/loopunroll/calleesave_main.i.dfy
@@ -1,9 +1,10 @@
-include "../../../obj/crypto/loopunroll/regions.gen.dfy"
+include "../../../obj/crypto/loopunroll/calleesave.gen.dfy"
 include "../../arch/x64/print.s.dfy"
 include "../../lib/util/Io.s.dfy"
 
 module CalleeSave {
 
+import opened CalleeSaveRestore
 import opened x64_print_s
 import opened Io_s
 
@@ -48,7 +49,6 @@ method {:main} Main(ghost env:HostEnvironment)
     }
 
     var win := (platform_choice == Win);
-
     printProcPlatform("CalleeSaveRestore",
        va_code_CalleeSaveRestore(),
         0, 0, asm_choice, platform_choice);
